\begin{align*}
    2xy' &= y + y' \\
    -y' + 2xy' &= y \\
    y'(-1 + 2x) &= y \\
    y' \frac{(-1 + 2x)}{(-1 + 2x)} &= \frac{1}{(-1 + 2x)} \cdot y \\
    y' &= \frac{1}{(-1 + 2x)} \cdot y
\end{align*}

\underline{Calcul de la solution generale :}

\begin{align*}
    y &= \lambda e^{-\int\frac{1}{\frac{1}{(-1+2x)}}},\quad \lambda \in \mathbb{R} \\
    &= \lambda e^{-\int (-1 + 2x)},\quad \lambda \in \mathbb{R}
\end{align*}

\underline{Calculons d'abord l'integrale :}

\begin{align*}
    -\int (-1 + 2x) &= -(-x + x^2) \\
    &= x - x^2
\end{align*}

\underline{Alors :}

\begin{align*}
    y &= \lambda e^{x - x^2},\quad \lambda \in \mathbb{R}
\end{align*}

\boxed{y = \lambda e^{x - x^2},\quad \lambda \in \mathbb{R}}