% \item $y' + y = 2e^x + 4 \sin(x)$
\underline{Etape 1: ESSM} \\
\begin{align*}
	y' + y &= 0 \\
	y' &= -y \\
	\frac{dy}{y} &= -1 \\
	\int \frac{1}{y} dy &= - \int 1 dx \\
	ln \lvert y \lvert &= -x + C, \quad C \in \mathbb{R} \\
	y &= -e^{-x}.e^C \\
	y &= \lambda e^{-x} \quad \text{(1)}
\end{align*}

\underline{Etape 2: EASM MVC} \\
\begin{align*}
	y' = -\lambda e^{-x}	 + \lambda'e^{-x} \\
	y' = e^{-x} (\lambda + \lambda') \text{(2)}
\end{align*}

\begin{align*}
	\text{(1) et (2) dans (E):} \\
	(-\lambda + \lambda)e^{-x} + \lambda e^{-x} &= 2e^x + 4\sin(x) \\
	\lambda' &= 2e^x + 4sin(x) \\
    \frac{d\lambda}{dx}e^{-x} &= 2e^x + 4sin(x) \\
    \int d\lambda &= \int (2e^{2x} + 4e^x \sin(x)) \, dx \\
    \int \, d\lambda &= \int 2e^{2x} \, dx + 4\int e^x \sin(x)) \, dx \\
    \int \, d\lambda &= e^{2x} + C + 4 [-\cos(x)e^x + \int e^x\cos(x)\, dx]
\end{align*}
Soit $I = \int e^x\cos(x)\ $ \\
\[
\left\{
\begin{aligned}
    u &= e^x \implies u'= e^x  \\
    v &= -\cos(x) \implies v' = \sin(x)
\end{aligned}
\right.
\]

$-\cos(x)e^x + \int e*x\cos(x)\, dx$
\[
\left\{
\begin{aligned}
    u &= e^x \implies v'= \cos(x)  \\
    u' &= e^x \implies v' = \sin(x)
\end{aligned}
\right.
\]

\begin{align*}
    -e^xcos(x) + -e^xsin(x) - \int e^x \sin(x)) \, dx \\
    -e^xcos(x) + -e^xsin(x) - I \\
    I &= e^x(sin(x) - cos(x)) - I \\
    2I &= e^x(sin(x) - cos(x)) \\
    I &= \frac{e^x}{2}(sin(x) - cos(x)) 
\end{align*}

% Ligne vaovao 
\begin{align*}
    \int \, d\lambda &= e^{2x} + c + 2e^x(sin(x) - cos(x)) + k \\
    \lambda x &= e^{2x} + e^{2x} (\sin(x) - \cos(x)) + C \\
    \lambda x &= e^{x} (e^{x} + 2(\sin(x) - \cos(x)) + C
\end{align*}

% Ligne vaovao
\begin{align*}
    y &= e^x.e^{-x} (e^{x} + 2(\sin(x) - \cos(x)) + Ce^{-x} \\
    y &= e^x + 2\sin(x) - 2\cos(x) + Ce^{-x}
\end{align*}
\boxed{y = e^x + 2\sin(x) - 2\cos(x) + Ce^{-x}, \quad C \in \mathbb{R}}