\begin{align*}
	\frac{x}{x}y' &= \frac{1}{x}y + \frac{3xy^2}{x} \\
	y' &= \frac{1}{x}y + 3y^2 \\
\end{align*}

$\text{On pose } z=y^{-1} = \frac{1}{y} \implies z'= - \frac{y'}{y^2}$

\begin{align*}
	-\frac{y'}{y^2} &= -\frac{1}{xy} - 3 \\
	\text{d'ou } z' &= -\frac{1}{x}z - 3 \\
	z' + \frac{1}{x}z &= -3 \quad (E)
\end{align*}

\underline{ESSM} \\
$z' + \frac{1}{x}z = 0$

\begin{align*}
	z_H &= \lambda e^{-\int \frac{1}{x}}, \quad \lambda \in \mathbb{R} \\
	    &= \lambda e^{-ln|x|} \\
	z_H &= \lambda \frac{1}{x}, \quad \lambda \in \mathbb{R}
\end{align*}

\underline{EASM} \\

\text{MVC: } \\
\begin{align*}
	t &= g(x)\frac{1}{x} \quad (1) \\
	t' &= \frac{g'(x)x - g(x)}{x^2} \quad (2)
\end{align*}

(1) et (2) dans (E) \\
\begin{align*}
	\frac{g'(x)x - g(x)}{x^2} + \frac{1}{x} g(x)\frac{1}{x} &= -3 \\
	\frac{g'(x)x}{x^2} - \frac{g(x)}{x^2} + \frac{g(x)}{x^2} &= -3 \\
	g'(x) &= -3x \\
	g(x) &= -\frac{3}{2}x^2 + C, \quad C \in \mathbb{R}
\end{align*}

\begin{align*}
	z_p &= (-\frac{3}{2} x^2 + C) \frac{1}{x} + \lambda(\frac{1}{x}) \\
	z_p &= (-\frac{3}{2}x + \psi(\frac{1}{x} + \frac{1}{x})), \quad \psi = \frac{C}{x} \\
	z_p &= -\frac{3}{2}x + \psi\frac{2}{x} \\
	z_p &= -\frac{3x^2 + 4\psi}{2x} \\
\end{align*}

$z = z_H + z_P \text{ et } y = y_H + y_P$ \\
$\text{or } z = \frac{1}{y} $ \\
$\text{Alors } y = \frac{1}{z_H} + \frac{1}{z_P} $
\boxed{y = \frac{x}{\lambda} + \frac{2x}{3x^2 + 4\psi}, \quad \lambda, \psi \in \mathbb{R}}