% \item $(x^2 + 1) y' + 3xy = x^2$ \\
		\underline{Etape 1: ESSM} \\
		\begin{align*}
			(x^2+1)y' + 3xy &= 0  \\
			(x^2+1)y' &= -3xy  \\
			(x^2+1) \frac{dy}{dx} &= -3xy \\
			(x^2-1) \frac{dy}{y} &= -3x \,dx \\
			\int \frac{1}{y} \, dy &= \int -\frac{3x}{x^2+1} \, dx
		\end{align*}
		Posons \\
		\[
		\left\{
		\begin{aligned}
			u &= x^2 + 1 \\
			u' &= 2x
		\end{aligned}
		\right.
		\]
		
		
		$\int -\frac{3x}{u} \, dx$ = $-3 \int \frac{x}{u} \, dx$ = $-3 \int \frac{du}{2u} $ = $\frac{-3}{2} \int \frac{du}{u}$ \\
		
		$\frac{du}{dx} = 2x \implies du=2xdx \implies xdx = \frac{du}{2}$ \\
		$\frac{-3}{2} \int \frac{du}{u}$ = -$\frac{3}{/2} ln \lvert u \lvert + C, \quad C \in \mathbb{R} $\\
		
		$ln \lvert y \lvert = -\frac{3}{2} ln \lvert x^2 + 1 \lvert + C$ \\
		$y = ke^{-\frac{3}{2}ln \lvert x^2 + 1 \lvert } \text{ avec } e^C = k$
		