\begin{align*}
	\frac{x}{x}y' &= \frac{1}{x}y + \frac{3xy^2}{x} \\
	y' &= \frac{1}{x}y + 3y^2 \\
\end{align*}

$\text{On pose } z=y^{-1} = \frac{1}{y} \implies z'= - \frac{y'}{y^2}$

\begin{align*}
	-\frac{y'}{y^2} &= -\frac{1}{xy} - 3 \\
	\text{d'ou } z' &= -\frac{1}{x}z - 3 \\
	z' + \frac{1}{x}z &= -3 \quad (E)
\end{align*}

\underline{ESSM} \\
$z' + \frac{1}{x}z = 0$

\begin{align*}
	z_H &= \lambda e^{-\int \frac{1}{x}}, \quad \lambda \in \mathbb{R} \\
	    &= \lambda e^{-ln|x|} \\
	z_H &= \lambda \frac{1}{x}, \quad \lambda \in \mathbb{R}
\end{align*}

\underline{EASM} \\

\text{MVC: } \\
\begin{align*}
	t &= g(x)\frac{1}{x} \quad (1) \\
	t' &= \frac{g'(x)x - g(x)}{x^2} \quad (2)
\end{align*}

\text{(1) et (2) dans (E)} \\
\begin{align*}
	\frac{g'(x)x - g(x)}{x^2} + \frac{1}{x} g(x)\frac{1}{x} &= -3 \\
	\frac{g'(x)x}{x^2} - \frac{g(x)}{x^2} + \frac{g(x)}{x^2} &= -3 \\
	g'(x) &= -3x \\
	g(x) &= -\frac{3}{2}x^ + C, \quad C \in \mathbb{R}
\end{align*}