\underline{C'est une equation de Bernoulli}
\begin{align*}
	\frac {y'}{y^3} + \frac{y}{(x+1)y^3} &= \frac{1}{2}(x+3)^3 \\
	\frac {y'}{y^3} + \frac{(x+1)^-1}{y^2} &= \frac{1}{2}(x+3)^3 \quad (E)\\ 
\end{align*}
\text{Changement de variable} \\
$u = \frac{1}{y^2} = y^{-2} \implies \frac{du}{dx} = -2y'y^{-3}$

\text{D'ou} \\ 
$(E1): \quad \frac{1}{-2}u' + (x+1)^{-1}u = \frac{1}{2}(x+1)^3 \quad (A)$

\underline{Etape 1: ESSM}
\begin{align}
	-\frac{1}{2}u' + (x+1)^{-1}u &= 0 \\
	\frac{1}{2}u' &= (x+1)^{-1}u \\
	\frac{du}{dx} &= 2(x+1)^{-1}u \\
	\frac{du}{u} &= 2(x+1)^{-1}dx \\
	\ln \lvert u \lvert &= 2 \ln \lvert x+1 \lvert + C, \quad C \in \mathbb{R} \\	
	\ln \lvert u \lvert &= \ln \lvert (x+1)^2 \lvert + C \\
	u &= e^{\ln \lvert (x+1)^2 \lvert} \times e^{C} \\
	u &= (x+1)^2 \times \lambda, \quad \lambda = e^{C} \quad (E1_1)
\end{align}

\underline{Etape 2: EASM}
\begin{align*}
	u' &= \lambda'(x+1)^2 + 2(x+1) \lambda \quad (E1_2)
\end{align*}

\text{$(E1_1)$ et $(E1_2)$ dans (E1)} \\
\begin{align*}
	-\frac{1}{2}[\lambda'(x+1)^2 + 2(x+1)\lambda] + (x+1)^{-1}(x+1)^2\lambda &= \frac{1}{2}(x+1)^3 \\
	-\frac{\lambda'}{2} (x+1)^2 - (x+1)\lambda + (x+1)\lambda &= \frac{1}{2}(x+1)^3 \\
	- \frac{\lambda'}{2} (x+1)^2 &= \frac{1}{2}(x+1)^3 \\
	\lambda' &= - (x+1) \\
	\frac{d\lambda}{dx}	 &= -(x+1) \\
	d\lambda &= -(x+1) dx \\
	\int \, d\lambda &= - \int (x+1) \, dx \\
	\lambda &= - (\frac{x^2}{2} + x) + K, \quad K \in \mathbb{R} \\	
\end{align*}

\text{La solution generale de (E1) est: }
$u = (- (\frac{x^2}{2} + x) + K) (x+1)^2$