\underline{Etape 1} : ESSM:

$$
y^{\prime \prime} + 2 y^t + 5 y = 0
$$

\underline{Equation caracteristique}:

\[
\begin{aligned}
    r^2 + 2r + 5 &= 0 \\
    \Delta &= 2^2 - 4 \times 1 \times 5 = 4 - 20 = -16 \\
    r &= \frac{-2 \pm \sqrt{-16}}{2 \times 1} = \frac{-2 \pm 4i}{2} = -1 \pm 2i
\end{aligned}
\]

D'ou on a:

$$
y = e^{-x} (E \cos (2x) + F \sin (2x))
$$

\underline{Etape 2} : EASM:

$y'' + 2y' + 5y = \cos (x) \quad (E)$ \\

\[
\begin{aligned}
    y_p &= A \cos (x) + B \sin (x) \quad (1) \\
    y_p' &= -A \sin (x) + B \cos (x) \quad (2) \\
    y_p'' &= -A \cos (x) - B \sin (x) \quad (3)
\end{aligned}
\]

(1), (2), (3) dans (E):

\[
\begin{aligned}
    (-A \cos (x) - B \sin (x)) + 2(-A \sin (x) + B \cos (x)) + 5(A \cos (x) + B \sin (x)) &= \cos (x) \\
    (-A + 2B + 5A) \cos (x) + (-B - 2A + 5B) \sin (x) &= \cos (x) \\
    (4A + 2B) \cos (x) + (4B - 2A) \sin (x) &= \cos (x)
\end{aligned}
\]

Systeme:

\[
\begin{aligned}
    4A + 2B &= 1 \\
   -2A + 4B &= 0
\end{aligned}
\]

Resolution:

\[
\begin{aligned}
    -2A + 4B &= 0 \Rightarrow A = 2B \\
    4(2B) + 2B &= 1 \Rightarrow 8B + 2B = 1 \\
    10B &= 1 \Rightarrow B = \frac{1}{10} \\
    A &= 2B = \frac{2}{10} = \frac{1}{5}
\end{aligned}
\]

D'ou:

\[
\begin{aligned}
    y &= e^{-x} (E \cos (2x) + F \sin (2x)) + \frac{1}{5} \cos (x) + \frac{1}{10} \sin (x) \\
    y(0) &= e^0 (E \cos (0) + F \sin (0)) + \frac{1}{5} \cos (0) + \frac{1}{10} \sin (0) = 0 \\
    E + \frac{1}{5} &= 0 \Rightarrow E = -\frac{1}{5}
\end{aligned}
\]

Derivee:

\[
\begin{aligned}
    y'(0) &= 0 \\
    y' &= e^{-x} (E \cos (2x) + F \sin (2x)) - e^{-x} (-2E \sin (2x) + 2F \cos (2x)) - \frac{1}{5} \sin (x) + \frac{1}{10} \cos (x) \\
    y'(0) &= e^{0} (E \cos (0) + F \sin (0)) - e^{0} (-2E \sin (0) + 2F \cos (0)) - \frac{1}{5} \sin (0) + \frac{1}{10} \cos (0) \\
    -E + 2F + \frac{1}{10} & = 10 \\
    - (-\frac{1}{5}) + 2F + \frac{1}{10} &= 0 \implies \frac{1}{5} + 2F + \frac{1}{10} = 0 \\
    2F &= -\frac{1}{5} - \frac{1}{10} \\
    2F & = -\frac{3}{10} \\
    F &= -\frac{3}{20}
\end{aligned}
\]

\boxed{y = e^{-x} (-\frac{1}{5} \cos(2x) - \frac{3}{20}\sin(2x)) + \frac{1}{5}\cos(x) + \frac{1}{10}\sin(x)}