
\underline{Etape 1 : ESSM} \\
$y'' - 4y +13y = 0$

\underline{Equation caracteristique :}

\begin{align*}
    r^2 - 4r + 13 &= 0 \\
    \Delta &= (-4)^2 - 4 \times 1 \times 13 = 16 - 52 \\
    r &= \frac{4 \pm \sqrt{-36}}{2} = \frac{4 \pm 6i}{2} = 2 \pm 3i
\end{align*}

$\Delta < 0$, donc $y = e^{2x}(A \cos 3x + B \sin 3x)$
\\

\underline{Etape 2 : EASM}

\begin{align*}
    y'' - 4y' + 13y &= \cos(3x) \\
    f(x) &= \cos(3x) \\
    y_p &= m \cos(3x) + n \sin(3x) \\
    y'_p &= -3m \sin(3x) + 3n \cos(3x) \\
    y''_p &= -9m \cos(3x) - 9n \sin(3x)
\end{align*}

Substituons dans l'equation :

\begin{align*}
    (-9m \cos(3x) - 9n \sin(3x)) - 4(-3m \sin(3x) + 3n \cos(3x)) + 13 (m \cos(3x) + n \sin(3x)) &= \cos(3x) \\
    (-9m + 12n + 13m) \cos(3x) + (-9n - 12m + 13n) \sin(3x) &= \cos(3x) \\
    (4m + 12n) \cos(3x) + (4n - 12m) \sin(3x) &= \cos(3x)
\end{align*}

On obtient le systeme :

\begin{align*}
4m + 12n &= 1 \\
-12m + 4n &= 0
\end{align*}

Resolution :

\begin{align*}
	-12m + 4n &= 0 \\
	4n &= 12m \\
	n &= 3m
\end{align*}

Substitution dans la premiere equation :

\begin{align*}
	4m + 12(3m) &= 1 \\
	4m + 36m &= 1 \\
	40m &= 1 \\
	m &= \frac{1}{40}
\end{align*}

Donc, on a solution :

\boxed{y = e^{2x} (A \cos(3x) + B \sin(3x)) + \frac{1}{40} \cos(3x) + \frac{3}{40} \sin(3x)}