\begin{align*}
	y'cos(2y) - sin(y) &= 0, \\
	y'cos(2y) &= sin(y)  \\
	y'\frac{cos(2y)}{cos(2y)} &= \frac{sin(y)}{cos(2y)} , \\
	y' &= \frac{sin(y)}{cos(2y)} or cos(2y) =  1-2cos(y) , \\
	y' &= \frac{sin(y)}{1-2cos^2(y)}  \\ \\
\end{align*}
	$ \text{Posons } u = cos(y)  $\\
	$ \text{Alors } \frac{du}{dy} = -sin(y) \Rightarrow dy = \frac{du}{-sin(y)} , $\\
	$ \text{On a alors }: y = \int \frac{sin(y)}{1-2u^2} \cdot \frac{du}{-sin(y)}  $\\
	$ y = \int\frac{1}{2u^2-1} $\\
	$ \text{Posons } w = \sqrt{2}u \Rightarrow u = \frac{w}{\sqrt{2}}  $\\
	$ \text{Alors }\frac{dw}{du} = \sqrt{2} \Rightarrow w = \frac{dw}{\sqrt{2}} $\\

\begin{align*}
	y &= \int\frac{1}{w^2-1} \cdot \frac{dw}{\sqrt{2}} \\
	y &= \frac{1}{\sqrt{2}}\int\frac{1}{w^2-1} dw \\
	y &= \frac{1}{\sqrt{2}}\int\frac{1}{(w-1)(w+1)} dw \\
\end{align*}


$ \text{\underline{Simplifions dabord la primitive}} $ \\
$ \frac{1}{(w-1)(w+1)} = \frac{A}{w-1} + \frac{B}{w+1} (E), \quad A, B \in\mathbb{R} , $ \\
$ \text{On multiplie chaque terme par (x-1)}  $ \\
$ \frac{1}{(w-1)} = A + \frac{B(w-1)}{(w+1)} $ \\
$ \text{Pour u = 1},  $ \\
$ \frac{1}{2} = A \quad (1) $ \\
$ \text{On multiplie chaque terme par (x+1)}  $ \\
$ \frac{1}{(w+1)} = \frac{A(w+1)}{(w-1)} + B $ \\
$ \text{Pour u = -1},  $ \\
$ -\frac{1}{2} = B \quad (2) $ \\

\text{(1) et (2) dans (E): } \\
\begin{align*}
	\frac{1}{(w-1)(w+1)} &= \frac{\frac{1}{2}}{(w-1)} + \frac{-\frac{1}{2}}{(w+1)} \\
	\frac{1}{(w-1)(w+1)} &= \frac{1}{2(w-1)} - \frac{1}{2(w+1)} \\
	\text{On a alors: } y &= \frac{1}{\sqrt{2}}[\int\frac{1}{2(w-1)} - \int\frac{1}{2(w+1)}] \\
\end{align*}

\begin{align*}
	y &= \frac{1}{\sqrt{2}}[\frac{1}{2}\int\frac{1}{(w-1)} - \frac{1}{2}\int\frac{1}{(w+1)}] \\
	y &= \frac{1}{2\sqrt{2}}[\int\frac{1}{(w-1)} - \int\frac{1}{(w+1)}] \\
	y &= \frac{\sqrt{2}}{4}[ln|w-1| + C - ln|w+1| + K], \quad C, K \in \mathbb{R} \\
	y &= \frac{\sqrt{2}}{4}[ln|w-1| - ln|w+1| + T], T \in \mathbb{R} \\
\end{align*}

\begin{align*}
	\text{\underline{Retour au changement de variable}} \\
	w = \sqrt{2}u \\
	\text{Alors } y &= \frac{\sqrt{2}}{4}(ln|\sqrt{2}u-1| - ln|\sqrt{2}u+1| + T), T \in \mathbb{R} \\
	u = cos(y) \\
	\text{Alors } y &= \frac{\sqrt{2}}{4}(ln|\sqrt{2}cos(y)-1| - ln|\sqrt{2}cos(y)+1| + T), T \in \mathbb{R}
\end{align*}
\boxed{y = \frac{\sqrt{2}}{4}(ln|\sqrt{2}cos(y)-1| - ln|\sqrt{2}cos(y)+1| + T), T \in \mathbb{R}}